diff --git a/Mathlib/Data/List/Join.lean b/Mathlib/Data/List/Join.lean index 7e97020ea8595..662b2562cbfa6 100644 --- a/Mathlib/Data/List/Join.lean +++ b/Mathlib/Data/List/Join.lean @@ -188,7 +188,7 @@ theorem join_drop_length_sub_one {L : List (List α)} (h : L ≠ []) : /-- We can rebracket `x ++ (l₁ ++ x) ++ (l₂ ++ x) ++ ... ++ (lₙ ++ x)` to `(x ++ l₁) ++ (x ++ l₂) ++ ... ++ (x ++ lₙ) ++ x` where `L = [l₁, l₂, ..., lₙ]`. -/ theorem append_join_map_append (L : List (List α)) (x : List α) : - x ++ (List.map (fun l => l ++ x) L).join = (List.map (fun l => x ++ l) L).join ++ x := by + x ++ (L.map (· ++ x)).join = (L.map (x ++ ·)).join ++ x := by induction' L with _ _ ih · rw [map_nil, join, append_nil, map_nil, join, nil_append] · rw [map_cons, join, map_cons, join, append_assoc, ih, append_assoc, append_assoc] @@ -196,7 +196,7 @@ theorem append_join_map_append (L : List (List α)) (x : List α) : /-- Reversing a join is the same as reversing the order of parts and reversing all parts. -/ theorem reverse_join (L : List (List α)) : - L.join.reverse = (List.map List.reverse L).reverse.join := by + L.join.reverse = (L.map reverse).reverse.join := by induction' L with _ _ ih · rfl · rw [join, reverse_append, ih, map_cons, reverse_cons', join_concat] @@ -204,14 +204,14 @@ theorem reverse_join (L : List (List α)) : /-- Joining a reverse is the same as reversing all parts and reversing the joined result. -/ theorem join_reverse (L : List (List α)) : - L.reverse.join = (List.map List.reverse L).join.reverse := by + L.reverse.join = (L.map reverse).join.reverse := by simpa [reverse_reverse, map_reverse] using congr_arg List.reverse (reverse_join L.reverse) #align list.join_reverse List.join_reverse -/-- Any member of `l : List (List α))` is a sublist of `l.join` -/ -lemma sublist_join (l : List (List α)) {s : List α} (hs : s ∈ l) : - List.Sublist s (l.join) := by - induction l with +/-- Any member of `L : List (List α))` is a sublist of `L.join` -/ +lemma sublist_join (L : List (List α)) {s : List α} (hs : s ∈ L) : + s.Sublist L.join := by + induction L with | nil => exfalso exact not_mem_nil s hs